project02/MessageType.v.dfy
@@ -1,8 +1,6 @@
 module MessageType {
   datatype Message =
 /*{*/
-    | Get(key: int, value: int)
-    | Put(key: int, value: int)
     | KeyValue(key: int, value: int, dest: nat, from: nat)
 /*}*/
 }
